13AssemblyCode/Assemble.thy
@@ -7,7 +7,7 @@ primrec assemble_op_len :: "byte_code \<Rightarrow> nat" where
 | "assemble_op_len (BPushCon k) = 7"
 | "assemble_op_len (BPushLam pc) = 11"
 | "assemble_op_len BApply = 21"
-| "assemble_op_len BReturn = 3"
+| "assemble_op_len BReturn = 2"
 | "assemble_op_len BJump = 18"
 
 primrec assemble_op :: "(nat \<Rightarrow> nat) \<Rightarrow> byte_code \<Rightarrow> assm list" where
@@ -15,7 +15,7 @@ primrec assemble_op :: "(nat \<Rightarrow> nat) \<Rightarrow> byte_code \<Righta
     AMov (Con 0),
     AAdd Vals 1,
     APutA Vals,
-    AGetA Env (Reg Vals),
+    AGetA Env (Reg Hp),
     ASubA 2 (Reg Env)] @
     concat (replicate x [
     AGetA Env (Reg Env),
@@ -34,13 +34,13 @@ primrec assemble_op :: "(nat \<Rightarrow> nat) \<Rightarrow> byte_code \<Righta
     APut Vals (Reg Hp)]"
 | "assemble_op mp (BPushLam pc) = [
     AAdd Hp 1, 
-    APut Hp (Con (mp pc)), 
+    APutPC Hp (mp pc), 
     AMov (Con 0),
     AAdd Hp 1, 
     APutA Hp,
     AAdd Hp 1, 
     APut Hp (Con 0),
-    AGetA Stk (Reg Hp), 
+    AGetA Stk (Reg Env), 
     ASubA 1 (Reg Stk),
     AMov (Reg Stk),
     AAdd Vals 1,
@@ -66,11 +66,10 @@ primrec assemble_op :: "(nat \<Rightarrow> nat) \<Rightarrow> byte_code \<Righta
     AMov PC,
     AAdd Env 1,
     APutA Env,
-    AGet Vals (Reg Env),
+    AGet Vals (Reg Hp),
     ASub Vals 1]"
 | "assemble_op mp BReturn = [
     AJmp,
-    APut Stk (Con 0),
     AGet Stk PC,
     ASub Stk 2]"
 | "assemble_op mp BJump = [
@@ -91,7 +90,7 @@ primrec assemble_op :: "(nat \<Rightarrow> nat) \<Rightarrow> byte_code \<Righta
     AMov (Reg Env),
     AAdd Env 1,
     APutA Env,
-    AGet Vals (Reg Env),
+    AGet Vals (Reg Hp),
     ASub Vals 1]"
 
 fun assembly_map :: "byte_code list \<Rightarrow> nat \<Rightarrow> nat" where
@@ -102,22 +101,31 @@ fun assembly_map :: "byte_code list \<Rightarrow> nat \<Rightarrow> nat" where
 definition assemble_code :: "byte_code list \<Rightarrow> assm list" where
   "assemble_code cd = concat (map (assemble_op (assembly_map cd)) cd)"
 
-definition assemble_heap :: "nat \<Rightarrow> (nat \<Rightarrow> nat) \<Rightarrow> (nat \<Rightarrow> nat) \<Rightarrow> nat \<Rightarrow> nat" where
-  "assemble_heap hp mp h x = (if x < hp \<and> x mod 3 = 2 \<and> h (x - 2) = 0 then mp (h x) else h x)"
+definition assemble_heap :: "(nat \<Rightarrow> nat) \<Rightarrow> (nat \<Rightarrow> nat) \<Rightarrow> nat \<Rightarrow> pseudoreg \<times> nat" where
+  "assemble_heap mp h x = (case x mod 3 of
+      0 \<Rightarrow> (Con 0, h x)
+    | Suc 0 \<Rightarrow> (if h (x - 1) = 0 then Reg Env else Con 0, h x)
+    | Suc (Suc 0) \<Rightarrow> if h (x - 2) = 0 then (PC, mp (h x)) else (Con 0, h x))"
 
-definition assemble_stack :: "nat \<Rightarrow> (nat \<Rightarrow> nat) \<Rightarrow> (nat \<Rightarrow> nat) \<Rightarrow> nat \<Rightarrow> nat" where
-  "assemble_stack sp mp s x = (if x < sp \<and> even x then mp (s x) else s x)"
+definition assemble_env :: "(nat \<Rightarrow> nat) \<Rightarrow> nat \<Rightarrow> pseudoreg \<times> nat" where
+  "assemble_env e x = (Reg (if even x then Hp else Env), e x)"
+
+definition assemble_vals :: "(nat \<Rightarrow> nat) \<Rightarrow> nat \<Rightarrow> pseudoreg \<times> nat" where
+  "assemble_vals vs x = (Reg Hp, vs x)"
+
+definition assemble_stack :: "(nat \<Rightarrow> nat) \<Rightarrow> (nat \<Rightarrow> nat) \<Rightarrow> nat \<Rightarrow> pseudoreg \<times> nat" where
+  "assemble_stack mp s x = (if even x then (PC, mp (s x)) else (Reg Env, s x))"
 
 primrec assemble_state :: "(nat \<Rightarrow> nat) \<Rightarrow> unstr_state \<Rightarrow> assm_state" where
   "assemble_state mp (US h hp e ep vs vp sh sp pc) = 
-    AS (case_register (assemble_heap hp mp h) e vs (assemble_stack sp mp sh)) 
-      (case_register hp ep vp sp) 0 (Con 0) (mp pc)"
+    AS (case_register (assemble_heap mp h) (assemble_env e) (assemble_vals vs) 
+      (assemble_stack mp sh)) (case_register hp ep vp sp) 0 (Con 0) (mp pc)"
 
-abbreviation assm_hp :: "nat \<Rightarrow> byte_code list \<Rightarrow> (nat \<Rightarrow> nat) \<Rightarrow> nat \<Rightarrow> nat" where
-  "assm_hp hp cd \<equiv> assemble_heap hp (assembly_map cd)"
+abbreviation assm_hp :: "byte_code list \<Rightarrow> (nat \<Rightarrow> nat) \<Rightarrow> nat \<Rightarrow> pseudoreg \<times> nat" where
+  "assm_hp cd \<equiv> assemble_heap (assembly_map cd)"
 
-abbreviation assm_stk :: "nat \<Rightarrow> byte_code list \<Rightarrow> (nat \<Rightarrow> nat) \<Rightarrow> nat \<Rightarrow> nat" where
-  "assm_stk sp cd \<equiv> assemble_stack sp (assembly_map cd)"
+abbreviation assm_stk :: "byte_code list \<Rightarrow> (nat \<Rightarrow> nat) \<Rightarrow> nat \<Rightarrow> pseudoreg \<times> nat" where
+  "assm_stk cd \<equiv> assemble_stack (assembly_map cd)"
 
 abbreviation assm_state :: "byte_code list \<Rightarrow> unstr_state \<Rightarrow> assm_state" where
   "assm_state cd \<equiv> assemble_state (assembly_map cd)"
@@ -245,12 +253,6 @@ lemma [simp]: "length (assemble_code cd) = list_sum (map (Suc \<circ> assemble_o
 lemma [simp]: "assembly_map cd (length cd) = length (assemble_code cd)"
   by (induction cd) (simp_all add: assemble_code_def)
 
-lemma [simp]: "assm_hp hp cd nmem = nmem"
-  by (auto simp add: assemble_heap_def)
-
-lemma [simp]: "assm_stk 0 cd m = m"
-  by (auto simp add: assemble_stack_def)
-
 lemma [simp]: "lookup (assemble_op mp op @ cd) (Suc (assemble_op_len op + x)) = lookup cd x"
 proof -
   have "lookup (assemble_op mp op @ cd) (length (assemble_op mp op) + x) = lookup cd x" 
@@ -295,20 +297,22 @@ lemma [simp]: "m Hp = h \<Longrightarrow> m Env = e \<Longrightarrow> m Vals = v
     m = case_register h e vs sh" 
   by rule (simp split: register.splits)
 
-lemma assm_hp_lemma1: "3 dvd x \<Longrightarrow> assemble_heap hp mp h x = h x"
+lemma assm_hp_lemma1: "3 dvd x \<Longrightarrow> assemble_heap mp h x = (Con 0, h x)"
   by (simp add: assemble_heap_def)
 
-lemma assm_hp_lemma2: "x mod 3 = 1 \<Longrightarrow> assemble_heap hp mp h x = h x"
+lemma assm_hp_lemma2: "x mod 3 = 1 \<Longrightarrow> h (x - 1) \<noteq> 0 \<Longrightarrow> assemble_heap mp h x = (Con 0, h x)"
   by (simp add: assemble_heap_def)
 
-lemma assm_hp_lemma3: "x mod 3 = 2 \<Longrightarrow> h (x - 2) \<noteq> 0 \<Longrightarrow> assemble_heap hp mp h x = h x"
+lemma assm_hp_lemma3: "x mod 3 = 1 \<Longrightarrow> h (x - 1) = 0 \<Longrightarrow>  assemble_heap mp h x = (Reg Env, h x)"
   by (simp add: assemble_heap_def)
 
-lemma assm_hp_lemma4: "x mod 3 = 2 \<Longrightarrow> h (x - 2) = 0 \<Longrightarrow> x < hp \<Longrightarrow> 
-    assemble_heap hp mp h x = mp (h x)"
+lemma assm_hp_lemma4: "x mod 3 = 2 \<Longrightarrow> h (x - 2) \<noteq> 0 \<Longrightarrow> assemble_heap mp h x = (Con 0, h x)"
   by (simp add: assemble_heap_def)
 
-lemma assemble_heap_update_lemma [simp]: "3 dvd hp \<Longrightarrow> x \<noteq> hp \<Longrightarrow> x \<noteq> Suc hp \<Longrightarrow> 
+lemma assm_hp_lemma5: "x mod 3 = 2 \<Longrightarrow> h (x - 2) = 0 \<Longrightarrow> assemble_heap mp h x = (PC, mp (h x))"
+  by (simp add: assemble_heap_def)
+
+lemma assemble_heap_update_lemma2 [simp]: "3 dvd hp \<Longrightarrow> x \<noteq> hp \<Longrightarrow> x \<noteq> Suc hp \<Longrightarrow> 
   x \<noteq> Suc (Suc hp) \<Longrightarrow> x mod 3 = 2 \<Longrightarrow> 
     (h(hp := a, Suc hp := b, Suc (Suc hp) := c)) (x - 2) = h (x - 2)"
 proof (induction x)
@@ -322,73 +326,82 @@ proof (induction x)
 qed simp_all
 
 lemma [simp]: "3 dvd hp \<Longrightarrow> x \<noteq> hp \<Longrightarrow> x \<noteq> Suc hp \<Longrightarrow> x \<noteq> Suc (Suc hp) \<Longrightarrow> 
-  assm_hp (Suc (Suc (Suc hp))) cd (h(hp := a, Suc hp := b, Suc (Suc hp) := c)) x = 
-    assm_hp hp cd h x"
-proof (unfold assemble_heap_def, cases "x mod 3 = 2")
-  case True
-  assume "3 dvd hp" and "x \<noteq> hp" and "x \<noteq> Suc hp" and "x \<noteq> Suc (Suc hp)"
-  moreover with True have "(h(hp := a, Suc hp := b, Suc (Suc hp) := c)) (x - 2) = h (x - 2)" 
-    by (metis assemble_heap_update_lemma)
-  ultimately show "(if x < Suc (Suc (Suc hp)) \<and> x mod 3 = 2 \<and> 
-    (h(hp := a, Suc hp := b, Suc (Suc hp) := c)) (x - 2) = 0
-      then assembly_map cd ((h(hp := a, Suc hp := b, Suc (Suc hp) := c)) x) 
-        else (h(hp := a, Suc hp := b, Suc (Suc hp) := c)) x) =
-          (if x < hp \<and> x mod 3 = 2 \<and> h (x - 2) = 0 then assembly_map cd (h x) else h x)" by simp
-next
-  case False
-  assume "x \<noteq> hp" and "x \<noteq> Suc hp" and "x \<noteq> Suc (Suc hp)"
-  hence "(x = hp \<longrightarrow> a = h hp) \<and> (x \<noteq> hp \<longrightarrow> (x = Suc hp \<longrightarrow> b = h (Suc hp)) \<and> 
-    (x \<noteq> Suc hp \<longrightarrow> x = Suc (Suc hp) \<longrightarrow> c = h (Suc (Suc hp))))" by simp
-  with False show "(if x < Suc (Suc (Suc hp)) \<and> x mod 3 = 2 \<and> 
-    (h(hp := a, Suc hp := b, Suc (Suc hp) := c)) (x - 2) = 0
-      then assembly_map cd ((h(hp := a, Suc hp := b, Suc (Suc hp) := c)) x) 
-        else (h(hp := a, Suc hp := b, Suc (Suc hp) := c)) x) =
-          (if x < hp \<and> x mod 3 = 2 \<and> h (x - 2) = 0 then assembly_map cd (h x) else h x)" by simp
-qed
+  assm_hp cd (h(hp := a, Suc hp := b, Suc (Suc hp) := c)) x = assm_hp cd h x"
+proof (cases "x mod 3")
+  case (Suc m) note S = Suc
+  assume A: "3 dvd hp" and B: "x \<noteq> hp" and C: "x \<noteq> Suc hp" and D: "x \<noteq> Suc (Suc hp)"
+  thus ?thesis 
+  proof (cases m)
+    case 0
+    from Suc C have X1: "x - 1 \<noteq> hp" by simp
+    from Suc D have X2: "x - 1 \<noteq> Suc hp" by simp
+    from Suc A 0 have X3: "x - 1 \<noteq> Suc (Suc hp)" by presburger
+    from B C D X1 X2 X3 have "(if (h(hp := a, Suc hp := b, Suc (Suc hp) := c)) (x - 1) = 0 
+      then Reg Env else Con 0, (h(hp := a, Suc hp := b, Suc (Suc hp) := c)) x) =
+        (if h (x - 1) = 0 then Reg Env else Con 0, h x)" 
+      by simp
+    with Suc 0 show ?thesis by (simp add: assemble_heap_def)
+  next
+    case (Suc m')
+    with S have M: "x mod 3 = Suc (Suc 0)" by simp
+    from D M have X1: "x - 2 \<noteq> hp" by simp
+    from A M have X2: "x - 2 \<noteq> Suc hp" by presburger
+    from A M have X3: "x - 2 \<noteq> Suc (Suc hp)" by presburger
+    from B C D X1 X2 X3 have "(if (h(hp := a, Suc hp := b, Suc (Suc hp) := c)) (x - 2) = 0
+         then (PC, assembly_map cd ((h(hp := a, Suc hp := b, Suc (Suc hp) := c)) x))
+         else (Con 0, (h(hp := a, Suc hp := b, Suc (Suc hp) := c)) x)) =
+    (if h (x - 2) = 0 then (PC, assembly_map cd (h x)) else (Con 0, h x))" by simp
+    with M show ?thesis by (simp add: assemble_heap_def)
+  qed
+qed (simp_all add: assemble_heap_def)
 
-lemma [simp]: "restructurable_heap h hp ep (length cd) \<Longrightarrow> 
-  (assm_hp hp cd h)(hp := Suc a, Suc hp := b, Suc (Suc hp) := c) = 
-    assm_hp (Suc (Suc (Suc hp))) cd (h(hp := Suc a, Suc hp := b, Suc (Suc hp) := c))"
+lemma [simp]: "restructurable_heap h hp ep (length cd) \<Longrightarrow> (assm_hp cd h)
+  (hp := (Con 0, Suc a), Suc hp := (Con 0, b), Suc (Suc hp) := (Con 0, c)) = 
+    assm_hp cd (h(hp := Suc a, Suc hp := b, Suc (Suc hp) := c))"
 proof
   fix x
   assume "restructurable_heap h hp ep (length cd)"
   hence H: "3 dvd hp" by (simp add: restructurable_heap_def)
   moreover hence "Suc hp mod 3 = 1" by presburger
   moreover hence "Suc (Suc hp) mod 3 = 2" by presburger
-  ultimately show "
-    ((assm_hp hp cd h)(hp := Suc a, Suc hp := b, Suc (Suc hp) := c)) x =
-      assm_hp (Suc (Suc (Suc hp))) cd (h(hp := Suc a, Suc hp := b, Suc (Suc hp) := c)) x" 
-    by (simp add: assm_hp_lemma1 assm_hp_lemma2 assm_hp_lemma3)
+  ultimately show "((assm_hp cd h)
+    (hp := (Con 0, Suc a), Suc hp := (Con 0, b), Suc (Suc hp) := (Con 0, c))) x =
+      assm_hp cd (h(hp := Suc a, Suc hp := b, Suc (Suc hp) := c)) x" 
+    by (simp add: assm_hp_lemma1 assm_hp_lemma2 assm_hp_lemma3 assm_hp_lemma4 assm_hp_lemma5)
 qed
 
-lemma [simp]: "restructurable_heap h hp ep (length cd) \<Longrightarrow> 
-  (assm_hp hp cd h)(hp := 0, Suc hp := a, Suc (Suc hp) := assembly_map cd b) = 
-    assm_hp (Suc (Suc (Suc hp))) cd (h(hp := 0, Suc hp := a, Suc (Suc hp) := b))"
+lemma [simp]: "restructurable_heap h hp ep (length cd) \<Longrightarrow> (assm_hp cd h)
+  (hp := (Con 0, 0), Suc hp := (Reg Env, a), Suc (Suc hp) := (PC, assembly_map cd b)) = 
+    assm_hp cd (h(hp := 0, Suc hp := a, Suc (Suc hp) := b))"
 proof
   fix x
   assume "restructurable_heap h hp ep (length cd)"
   hence H: "3 dvd hp" by (simp add: restructurable_heap_def)
   moreover hence "Suc hp mod 3 = 1" by presburger
   moreover hence "Suc (Suc hp) mod 3 = 2" by presburger
-  ultimately show "((assm_hp hp cd h)(hp := 0, Suc hp := a, 
-    Suc (Suc hp) := assembly_map cd b)) x =
-      assm_hp (Suc (Suc (Suc hp))) cd (h(hp := 0, Suc hp := a, Suc (Suc hp) := b)) x" 
-    by (simp add: assm_hp_lemma1 assm_hp_lemma2 assm_hp_lemma4)
+  ultimately show "((assm_hp cd h)(hp := (Con 0, 0), Suc hp := (Reg Env, a), 
+    Suc (Suc hp) := (PC, assembly_map cd b))) x =
+      assm_hp cd (h(hp := 0, Suc hp := a, Suc (Suc hp) := b)) x" 
+    by (simp add: assm_hp_lemma1 assm_hp_lemma2 assm_hp_lemma3 assm_hp_lemma4 assm_hp_lemma5)
 qed
 
 lemma [simp]: "restructurable_vals vs (Suc (Suc vp)) hp \<Longrightarrow> 
-    assemble_heap hp mp h (Suc (vs vp)) = h (Suc (vs vp))"
+  assemble_heap mp h (Suc (vs vp)) = (if h (vs vp) = 0 then Reg Env else Con 0, h (Suc (vs vp)))"
 proof (unfold assemble_heap_def restructurable_vals_def)
   assume "\<forall>x<Suc (Suc vp). 3 dvd vs x \<and> vs x < hp"
   hence "3 dvd vs vp" by simp
   hence "Suc (vs vp) mod 3 = 1" by presburger
-  thus "(if Suc (vs vp) < hp \<and> Suc (vs vp) mod 3 = 2 \<and> h (Suc (vs vp) - 2) = 0 
-         then mp (h (Suc (vs vp))) else h (Suc (vs vp))) = h (Suc (vs vp))" by simp
+  thus "(case Suc (vs vp) mod 3 of 0 \<Rightarrow> (Con 0, h (Suc (vs vp)))
+     | Suc 0 \<Rightarrow> (if h (Suc (vs vp) - 1) = 0 then Reg Env else Con 0, h (Suc (vs vp)))
+     | Suc (Suc 0) \<Rightarrow> if h (Suc (vs vp) - 2) = 0 then (PC, mp (h (Suc (vs vp)))) 
+        else (Con 0, h (Suc (vs vp)))
+     | Suc (Suc (Suc x)) \<Rightarrow> nmem x) =
+    (if h (vs vp) = 0 then Reg Env else Con 0, h (Suc (vs vp)))" by simp
 qed
 
 lemma [simp]: "restructurable_vals vs (Suc (Suc vp)) hp \<Longrightarrow> h (vs vp) = 0 \<Longrightarrow> 
   restructurable_heap h hp ep lcd \<Longrightarrow>
-    assemble_heap hp mp h (Suc (Suc (vs vp))) = mp (h (Suc (Suc (vs vp))))"
+    assemble_heap mp h (Suc (Suc (vs vp))) = (PC, mp (h (Suc (Suc (vs vp)))))"
 proof (unfold assemble_heap_def restructurable_vals_def)
   assume "\<forall>x<Suc (Suc vp). 3 dvd vs x \<and> vs x < hp"
   hence "3 dvd vs vp \<and> vs vp < hp" by simp
@@ -396,78 +409,94 @@ proof (unfold assemble_heap_def restructurable_vals_def)
   moreover hence "3 dvd hp" by auto
   ultimately have "Suc (Suc (vs vp)) mod 3 = 2 \<and> Suc (Suc (vs vp)) < hp" by presburger
   moreover assume "h (vs vp) = 0"
-  ultimately show "(if Suc (Suc (vs vp)) < hp \<and> Suc (Suc (vs vp)) mod 3 = 2 \<and> 
-    h (Suc (Suc (vs vp)) - 2) = 0 then mp (h (Suc (Suc (vs vp)))) 
-      else h (Suc (Suc (vs vp)))) = mp (h (Suc (Suc (vs vp))))" 
+  ultimately show "(case Suc (Suc (vs vp)) mod 3 of 0 \<Rightarrow> (Con 0, h (Suc (Suc (vs vp))))
+     | Suc 0 \<Rightarrow> (if h (Suc (Suc (vs vp)) - 1) = 0 then Reg Env else Con 0, h (Suc (Suc (vs vp))))
+     | Suc (Suc 0) \<Rightarrow>
+         if h (Suc (Suc (vs vp)) - 2) = 0 then (PC, mp (h (Suc (Suc (vs vp))))) 
+        else (Con 0, h (Suc (Suc (vs vp))))
+     | Suc (Suc (Suc x)) \<Rightarrow> nmem x) =
+    (PC, mp (h (Suc (Suc (vs vp)))))" 
         by simp
-qed
+    qed
 
-lemma [simp]: "h (vs vp) = Suc x \<Longrightarrow>
-    assemble_heap hp mp h (Suc (Suc (vs vp))) = h (Suc (Suc (vs vp)))"
-  by (simp add: assemble_heap_def)
+lemma [simp]: "Suc (Suc (vs vp)) mod 3 \<noteq> Suc (Suc (Suc x))" 
+  by simp
 
-lemma [simp]: "even sp \<Longrightarrow> assm_stk (Suc (Suc sp)) cd sh (Suc sp) = sh (Suc sp)"
+lemma [simp]: "h (vs vp) = Suc x \<Longrightarrow> vs vp mod 3 = 0 \<Longrightarrow>
+    assemble_heap mp h (Suc (Suc (vs vp))) = (Con 0, h (Suc (Suc (vs vp))))"
+  by (simp add: assemble_heap_def split: nat.splits) presburger
+
+lemma [simp]: "even sp \<Longrightarrow> assm_stk cd sh (Suc sp) = (Reg Env, sh (Suc sp))"
   by (simp add: assemble_stack_def)
 
-lemma [simp]: "even sp \<Longrightarrow> ((assm_stk sp cd sh)(sp := assembly_map cd pc, Suc sp := a)) = 
-    (assm_stk (Suc (Suc sp)) cd (sh(sp := pc, Suc sp := a)))"
+lemma [simp]: "even sp \<Longrightarrow> 
+  (assm_stk cd sh)(sp := (PC, assembly_map cd pc), Suc sp := (Reg Env, a)) = 
+    (assm_stk cd (sh(sp := pc, Suc sp := a)))"
   by (auto simp add: assemble_stack_def)
 
 lemma [simp]: "even (Suc sp) \<Longrightarrow> 
-  (assm_stk (Suc sp) cd sh)(Suc sp := assembly_map cd pc, Suc (Suc sp) := k) =
-    (assm_stk (Suc (Suc (Suc sp))) cd (sh(Suc sp := pc, Suc (Suc sp) := k)))"
+  (assm_stk cd sh)(Suc sp := (PC, assembly_map cd pc), Suc (Suc sp) := (Reg Env, k)) =
+    (assm_stk cd (sh(Suc sp := pc, Suc (Suc sp) := k)))"
   by (auto simp add: assemble_stack_def)
 
 lemma [simp]: "even (Suc sp) \<Longrightarrow> 
-    (assm_stk (Suc sp) cd sh)(sp := k) = assm_stk (Suc sp) cd (sh(sp := k))"
+    (assm_stk cd sh)(sp := (Reg Env, k)) = assm_stk cd (sh(sp := k))"
   by (auto simp add: assemble_stack_def)
 
 lemma [simp]: "even (Suc (Suc sp)) \<Longrightarrow> 
-    ((assm_stk (Suc (Suc sp)) cd sh)(sp := 0)) = assm_stk sp cd (sh(sp := 0))"
+    (assm_stk cd sh)(sp := (PC, 0)) = assm_stk cd (sh(sp := 0))"
   by rule (auto simp add: assemble_stack_def)
 
-lemma [simp]: "even (Suc sp) \<Longrightarrow> assm_stk (Suc sp) cd sh sp = sh sp"
+lemma [simp]: "even (Suc sp) \<Longrightarrow> assm_stk cd sh sp = (Reg Env, sh sp)"
   by (simp add: assemble_stack_def)
 
-lemma [simp]: "even (Suc (Suc sp)) \<Longrightarrow> assm_stk (Suc (Suc sp)) cd sh sp = assembly_map cd (sh sp)"
+lemma [simp]: "even (Suc (Suc sp)) \<Longrightarrow> assm_stk cd sh sp = 
+    (PC, assembly_map cd (sh sp))"
   by (simp add: assemble_stack_def)
 
-lemma [simp]: "assm_stk 2 cd (sh(0 := 0, Suc 0 := 0)) = (sh(0 := 0, Suc 0 := 0))"
-  by (auto simp add: assemble_stack_def)
+lemma [simp]: "(assemble_vals vs)(vp := (Reg Hp, y)) = assemble_vals (vs(vp := y))"
+  by (auto simp add: assemble_vals_def)
+
+lemma [simp]: "even ep \<Longrightarrow> (assemble_env e)(ep := (Reg Hp, a), Suc ep := (Reg Env, b)) = 
+    assemble_env (e(ep := a, Suc ep := b))"
+  by (auto simp add: assemble_env_def)
 
 lemma [simp]: "unstr_lookup e a x = Some v \<Longrightarrow> lookup cd pc = Some (BLookup y) \<Longrightarrow> x \<le> y \<Longrightarrow> 
   pc < length cd \<Longrightarrow> iter_evala (assemble_code cd) (5 + 2 * x) 
-    (AS (case_register h e vs sh) (case_register hp ep vp sp) a (Reg Env)
-      (5 + 2 * x + assembly_map cd pc)) = Some (AS (case_register h e (vs(vp := v)) sh)  
-        (case_register hp ep (Suc vp) sp) 0 (Con 0) (assembly_map cd pc))"
+    (AS (case_register h (assemble_env e) vs sh) (case_register hp ep vp sp) a (Reg Env)
+      (5 + 2 * x + assembly_map cd pc)) = Some (AS (case_register h (assemble_env e)
+        (vs(vp := (Reg Hp, v))) sh) (case_register hp ep (Suc vp) sp) 0 (Con 0) 
+          (assembly_map cd pc))"
 proof (induction e a x rule: unstr_lookup.induct)
   case (3 e p)
   moreover from 3 have "lookup (assemble_code cd) (4 + assembly_map cd pc) = 
     Some (ASubA 2 (Reg Env))" by simp
   moreover from 3 have "lookup (assemble_code cd) (3 + assembly_map cd pc) = 
-    Some (AGetA Env (Reg Vals))" by simp
+    Some (AGetA Env (Reg Hp))" by simp
   moreover from 3 have "lookup (assemble_code cd) (2 + assembly_map cd pc) = 
-    Some (APutA Vals)" by (simp del: add_2_eq_Suc) (simp add: numeral_def)
-  ultimately show ?case by (simp add: numeral_def)
+    Some (APutA Vals)" by (simp del: add_2_eq_Suc)
+  ultimately show ?case by (simp add: numeral_def assemble_env_def split: if_splits)
 next
   case (4 e p x)
-  hence "lookup (assemble_code cd) (6 + 2 * x + assembly_map cd pc) = 
+  moreover hence "lookup (assemble_code cd) (6 + 2 * x + assembly_map cd pc) = 
     Some (ASubA (Suc 0) (Reg Env))" by simp
   moreover from 4 have "lookup (assemble_code cd) (5 + 2 * x + assembly_map cd pc) = 
     Some (AGetA Env (Reg Env))" by simp
   ultimately have "iter_evala (assemble_code cd) 2
-    (AS (case_register h e vs sh) (case_register hp ep vp sp) (Suc (Suc p)) (Reg Env)
-      (7 + 2 * x + assembly_map cd pc)) = Some (AS (case_register h e vs sh) 
+    (AS (case_register h (assemble_env e) vs sh) (case_register hp ep vp sp) (Suc (Suc p)) (Reg Env)
+      (7 + 2 * x + assembly_map cd pc)) = Some (AS (case_register h (assemble_env e) vs sh) 
         (case_register hp ep vp sp) (e (Suc p)) (Reg Env) (5 + 2 * x + assembly_map cd pc))" 
-    by (simp add: numeral_def)
+    by (simp add: numeral_def assemble_env_def split: if_splits) presburger
   moreover from 4 have "iter_evala (assemble_code cd) (5 + 2 * x) 
-    (AS (case_register h e vs sh) (case_register hp ep vp sp) (e (Suc p)) (Reg Env)
-      (5 + 2 * x + assembly_map cd pc)) = Some (AS (case_register h e (vs(vp := v)) sh) 
-        (case_register hp ep (Suc vp) sp) 0 (Con 0) (assembly_map cd pc))" by simp 
+    (AS (case_register h (assemble_env e) vs sh) (case_register hp ep vp sp) (e (Suc p)) (Reg Env)
+      (5 + 2 * x + assembly_map cd pc)) = Some (AS (case_register h (assemble_env e) 
+        (vs(vp := (Reg Hp, v))) sh) (case_register hp ep (Suc vp) sp) 0 (Con 0) 
+          (assembly_map cd pc))" by (simp split: if_splits)
   ultimately have "iter_evala (assemble_code cd) (2 + (5 + 2 * x))
-    (AS (case_register h e vs sh) (case_register hp ep vp sp) (Suc (Suc p)) (Reg Env)
-      (7 + 2 * x + assembly_map cd pc)) = Some (AS (case_register h e (vs(vp := v)) sh)
-        (case_register hp ep (Suc vp) sp) 0 (Con 0) (assembly_map cd pc))" 
+    (AS (case_register h (assemble_env e) vs sh) (case_register hp ep vp sp) (Suc (Suc p)) (Reg Env)
+      (7 + 2 * x + assembly_map cd pc)) = Some (AS (case_register h (assemble_env e) 
+        (vs(vp := (Reg Hp, v))) sh) (case_register hp ep (Suc vp) sp) 0 (Con 0) 
+          (assembly_map cd pc))" 
     using iter_evala_combine by blast
   thus ?case by simp
 qed simp_all
@@ -484,27 +513,29 @@ proof (induction cd\<^sub>b \<Sigma>\<^sub>u \<Sigma>\<^sub>u' rule: evalu.induc
   moreover from evu_lookup have "lookup (assemble_code cd) (5 + 2 * x + assembly_map cd pc) = 
     Some (AGetA Stk (Reg Env))" by simp
   ultimately have "iter_evala (assemble_code cd) 3 
-    (AS (case_register (assm_hp hp cd h) e vs (assm_stk (Suc sp) cd sh)) 
-      (case_register hp ep vp (Suc sp)) 0 (Con 0) (8 + 2 * x + assembly_map cd pc)) = 
-        Some (AS (case_register (assm_hp hp cd h) e vs (assm_stk (Suc sp) cd sh)) 
-          (case_register hp ep vp (Suc sp)) (sh sp) (Reg Env) (5 + 2 * x + assembly_map cd pc))" 
+    (AS (case_register (assm_hp cd h) (assemble_env e) (assemble_vals vs) 
+      (assm_stk cd sh)) (case_register hp ep vp (Suc sp)) 0 (Con 0) 
+        (8 + 2 * x + assembly_map cd pc)) = Some (AS (case_register (assm_hp cd h) 
+          (assemble_env e) (assemble_vals vs) (assm_stk cd sh)) 
+            (case_register hp ep vp (Suc sp)) (sh sp) (Reg Env) (5 + 2 * x + assembly_map cd pc))" 
     by (simp add: numeral_def)
   moreover from evu_lookup have "iter_evala (assemble_code cd) (5 + 2 * x) 
-    (AS (case_register (assm_hp hp cd h) e vs (assm_stk (Suc sp) cd sh)) 
+    (AS (case_register (assm_hp cd h) (assemble_env e) (assemble_vals vs) (assm_stk cd sh)) 
       (case_register hp ep vp (Suc sp)) (sh sp) (Reg Env) (5 + 2 * x + assembly_map cd pc)) = 
-        Some (AS (case_register (assm_hp hp cd h) e (vs(vp := y)) (assm_stk (Suc sp) cd sh)) 
-          (case_register hp ep (Suc vp) (Suc sp)) 0 (Con 0) (assembly_map cd pc))" by simp
+        Some (AS (case_register (assm_hp cd h) (assemble_env e) (assemble_vals (vs(vp := y))) 
+          (assm_stk cd sh)) (case_register hp ep (Suc vp) (Suc sp)) 0 (Con 0) (assembly_map cd pc))" 
+    by simp
   ultimately have "iter_evala (assemble_code cd) (3 + (5 + 2 * x)) 
-    (AS (case_register (assm_hp hp cd h) e vs (assm_stk (Suc sp) cd sh)) 
+    (AS (case_register (assm_hp cd h) (assemble_env e) (assemble_vals vs) (assm_stk cd sh)) 
       (case_register hp ep vp (Suc sp)) 0 (Con 0) (8 + 2 * x + assembly_map cd pc)) = 
-        Some (AS (case_register (assm_hp hp cd h) e (vs(vp := y)) (assm_stk (Suc sp) cd sh)) 
-          (case_register hp ep (Suc vp) (Suc sp)) 0 (Con 0) (assembly_map cd pc))" 
+        Some (AS (case_register (assm_hp cd h) (assemble_env e) (assemble_vals (vs(vp := y))) 
+          (assm_stk cd sh)) (case_register hp ep (Suc vp) (Suc sp)) 0 (Con 0) (assembly_map cd pc))" 
     using iter_evala_combine by blast
   hence "iter_evala (assemble_code cd) (3 + (5 + 2 * x)) 
-    (AS (case_register (assm_hp hp cd h) e vs (assm_stk (Suc sp) cd sh)) 
+    (AS (case_register (assm_hp cd h) (assemble_env e) (assemble_vals vs) (assm_stk cd sh)) 
       (case_register hp ep vp (Suc sp)) 0 (Con 0) (8 + (2 * x + assembly_map cd pc))) = 
-        Some (AS (case_register (assm_hp hp cd h) e (vs(vp := y)) (assm_stk (Suc sp) cd sh)) 
-          (case_register hp ep (Suc vp) (Suc sp)) 0 (Con 0) (assembly_map cd pc))"
+        Some (AS (case_register (assm_hp cd h) (assemble_env e) (assemble_vals (vs(vp := y))) 
+          (assm_stk cd sh)) (case_register hp ep (Suc vp) (Suc sp)) 0 (Con 0) (assembly_map cd pc))"
     by (metis add.assoc)
   with evu_lookup show ?case by auto
 next
@@ -520,12 +551,13 @@ next
   moreover from evu_pushcon have "lookup (assemble_code cd) (3 + assembly_map cd pc) = 
     Some (APut Hp (Con k))" by simp 
   moreover from evu_pushcon have "lookup (assemble_code cd) (2 + assembly_map cd pc) = 
-    Some (AAdd Hp 1)" by (simp del: add_2_eq_Suc) (simp add: numeral_def)
-  ultimately have "iter_evala (assemble_code cd) 8 (AS (case_register (assm_hp hp cd h) e vs 
-    (assm_stk (Suc sp) cd sh)) (case_register hp ep vp (Suc sp)) 0 (Con 0)
-      (assembly_map cd (Suc pc))) = Some (AS (case_register (assm_hp (3 + hp) cd (h(hp := 1,
-        Suc hp := k, Suc (Suc hp) := 0))) e (vs(vp := hp)) (assm_stk (Suc sp) cd sh)) 
-          (case_register (3 + hp) ep (Suc vp) (Suc sp)) 0 (Con 0) (assembly_map cd pc))" 
+    Some (AAdd Hp 1)" by (simp del: add_2_eq_Suc)
+  ultimately have "iter_evala (assemble_code cd) 8 (AS (case_register (assm_hp cd h) 
+    (assemble_env e) (assemble_vals vs) (assm_stk cd sh)) (case_register hp ep vp (Suc sp)) 0 
+      (Con 0) (assembly_map cd (Suc pc))) = Some (AS (case_register (assm_hp cd (h(hp := 1,
+        Suc hp := k, Suc (Suc hp) := 0))) (assemble_env e) (assemble_vals (vs(vp := hp))) 
+          (assm_stk cd sh)) (case_register (3 + hp) ep (Suc vp) (Suc sp)) 0 (Con 0) 
+            (assembly_map cd pc))" 
     by (auto simp add: numeral_def)
   thus ?case by auto
 next
@@ -539,7 +571,7 @@ next
   moreover from evu_pushlam have "lookup (assemble_code cd) (8 + assembly_map cd pc) = 
     Some (ASubA 1 (Reg Stk))" by simp
   moreover from evu_pushlam have "lookup (assemble_code cd) (7 + assembly_map cd pc) = 
-    Some (AGetA Stk (Reg Hp))" by simp
+    Some (AGetA Stk (Reg Env))" by simp
   moreover from evu_pushlam have "lookup (assemble_code cd) (6 + assembly_map cd pc) = 
     Some (APut Hp (Con 0))" by simp
   moreover from evu_pushlam have "lookup (assemble_code cd) (5 + assembly_map cd pc) = 
@@ -549,20 +581,22 @@ next
   moreover from evu_pushlam have "lookup (assemble_code cd) (3 + assembly_map cd pc) = 
     Some (AAdd Hp 1)" by simp
   moreover from evu_pushlam have "lookup (assemble_code cd) (2 + assembly_map cd pc) = 
-    Some (AMov (Con 0))" by (simp del: add_2_eq_Suc) (simp add: numeral_def)
-  ultimately have "iter_evala (assemble_code cd) 12 (AS (case_register (assm_hp hp cd h) e vs 
-    (assm_stk (Suc sp) cd sh)) (case_register hp ep vp (Suc sp)) 0 (Con 0)
-      (assembly_map cd (Suc pc))) = Some (AS (case_register (assm_hp (3 + hp) cd (h(hp := 0, 
-        Suc hp := sh sp, Suc (Suc hp) := pc'))) e (vs(vp := hp)) (assm_stk (Suc sp) cd sh)) 
-        (case_register (3 + hp) ep (Suc vp) (Suc sp)) 0 (Con 0) (assembly_map cd pc))" 
+    Some (AMov (Con 0))" by (simp del: add_2_eq_Suc)
+  ultimately have "iter_evala (assemble_code cd) 12 (AS (case_register (assm_hp cd h) 
+    (assemble_env e) (assemble_vals vs) (assm_stk cd sh)) (case_register hp ep vp (Suc sp)) 0 
+      (Con 0) (assembly_map cd (Suc pc))) = Some (AS (case_register (assm_hp cd (h(hp := 0, 
+        Suc hp := sh sp, Suc (Suc hp) := pc'))) (assemble_env e) (assemble_vals (vs(vp := hp))) 
+          (assm_stk cd sh)) (case_register (3 + hp) ep (Suc vp) (Suc sp)) 0 (Con 0) 
+            (assembly_map cd pc))" 
     by (auto simp add: numeral_def)
   thus ?case by auto
 next
   case (evu_apply cd pc h vs vp hp e ep sh sp)
+  moreover hence "even ep" by auto
   moreover from evu_apply have "lookup (assemble_code cd) (21 + assembly_map cd pc) = 
     Some (ASub Vals 1)" by simp
   moreover from evu_apply have "lookup (assemble_code cd) (20 + assembly_map cd pc) = 
-    Some (AGet Vals (Reg Env))" by simp
+    Some (AGet Vals (Reg Hp))" by simp
   moreover from evu_apply have "lookup (assemble_code cd) (19 + assembly_map cd pc) = 
     Some (APutA Env)" by simp
   moreover from evu_apply have "lookup (assemble_code cd) (18 + assembly_map cd pc) = 
@@ -598,35 +632,34 @@ next
   moreover from evu_apply have "lookup (assemble_code cd) (3 + assembly_map cd pc) = 
     Some (AGet Vals (Reg Hp))" by simp
   moreover from evu_apply have "lookup (assemble_code cd) (2 + assembly_map cd pc) = 
-    Some (AAddA 2 (Reg Hp))" by (simp del: add_2_eq_Suc) (simp add: numeral_def)
-  ultimately have "iter_evala (assemble_code cd) 22 (AS (case_register (assm_hp hp cd h) e vs 
-    (assm_stk (Suc sp) cd sh)) (case_register hp ep (Suc (Suc vp)) (Suc sp)) 0 (Con 0)
-      (assembly_map cd (Suc pc))) = Some (AS (case_register (assm_hp hp cd h) 
-        (e(ep := vs (Suc vp), Suc ep := h (Suc (vs vp)))) vs (assm_stk (Suc (Suc (Suc sp))) cd 
-          (sh(Suc sp := pc, Suc (Suc sp) := Suc (Suc ep))))) (case_register hp 
+    Some (AAddA 2 (Reg Hp))" by (simp del: add_2_eq_Suc)
+  ultimately have "iter_evala (assemble_code cd) 22 (AS (case_register (assm_hp cd h) 
+    (assemble_env e) (assemble_vals vs) (assm_stk cd sh)) (case_register hp ep (Suc (Suc vp)) 
+      (Suc sp)) 0 (Con 0) (assembly_map cd (Suc pc))) = Some (AS (case_register (assm_hp cd h) 
+        (assemble_env (e(ep := vs (Suc vp), Suc ep := h (Suc (vs vp))))) (assemble_vals vs) 
+          (assm_stk cd (sh(Suc sp := pc, Suc (Suc sp) := Suc (Suc ep))))) (case_register hp 
             (Suc (Suc ep)) vp (Suc (Suc (Suc sp)))) 0 (Con 0) 
               (assembly_map cd (h (Suc (Suc (vs vp))))))"
-    by (auto simp add: numeral_def)
+    by (auto simp add: numeral_def assemble_vals_def)
   thus ?case by auto
 next
   case (evu_return cd pc h hp e ep vs vp sh sp)
-  moreover from evu_return have "lookup (assemble_code cd) (3 + assembly_map cd pc) = 
-    Some (ASub Stk 2)" by simp
   moreover from evu_return have "lookup (assemble_code cd) (2 + assembly_map cd pc) = 
-    Some (AGet Stk PC)" by (simp del: add_2_eq_Suc) (simp add: numeral_def)
-  ultimately have "iter_evala (assemble_code cd) 4 (AS (case_register (assm_hp hp cd h) e vs 
-    (assm_stk (Suc (Suc sp)) cd sh)) (case_register hp ep vp (Suc (Suc sp))) 0 (Con 0)
-      (assembly_map cd (Suc pc))) = Some (AS (case_register (assm_hp hp cd h) e vs 
-        (assm_stk sp cd (sh(sp := 0)))) (case_register hp ep vp sp) 0 (Con 0)
+    Some (ASub Stk 2)" by (simp del: add_2_eq_Suc)
+  ultimately have "iter_evala (assemble_code cd) 3 (AS (case_register (assm_hp cd h) 
+    (assemble_env e) (assemble_vals vs) (assm_stk cd sh)) (case_register hp ep vp (Suc (Suc sp))) 0 
+      (Con 0) (assembly_map cd (Suc pc))) = Some (AS (case_register (assm_hp cd h) (assemble_env e) 
+        (assemble_vals vs) (assm_stk cd sh)) (case_register hp ep vp sp) 0 (Con 0)
           (assembly_map cd (sh sp)))"
     by (simp add: numeral_def)
   thus ?case by auto
 next
   case (evu_jump cd pc h vs vp hp e ep sh sp)
+  moreover hence "even ep" by auto
   moreover from evu_jump have "lookup (assemble_code cd) (18 + assembly_map cd pc) = 
     Some (ASub Vals 1)" by simp
   moreover from evu_jump have "lookup (assemble_code cd) (17 + assembly_map cd pc) = 
-    Some (AGet Vals (Reg Env))" by simp
+    Some (AGet Vals (Reg Hp))" by simp
   moreover from evu_jump have "lookup (assemble_code cd) (16 + assembly_map cd pc) = 
     Some (APutA Env)" by simp
   moreover from evu_jump have "lookup (assemble_code cd) (15 + assembly_map cd pc) = 
@@ -656,14 +689,14 @@ next
   moreover from evu_jump have "lookup (assemble_code cd) (3 + assembly_map cd pc) = 
     Some (AGet Vals (Reg Hp))" by simp
   moreover from evu_jump have "lookup (assemble_code cd) (2 + assembly_map cd pc) = 
-    Some (AAddA 2 (Reg Hp))" by (simp del: add_2_eq_Suc) (simp add: numeral_def)
-  ultimately have "iter_evala (assemble_code cd) 19 (AS (case_register (assm_hp hp cd h) e vs 
-    (assm_stk (Suc sp) cd sh)) (case_register hp ep (Suc (Suc vp)) (Suc sp)) 0 (Con 0)
-      (assembly_map cd (Suc pc))) = Some (AS (case_register (assm_hp hp cd h) 
-        (e(ep := vs (Suc vp), Suc ep := h (Suc (vs vp)))) vs (assm_stk (Suc sp) cd 
-          (sh(sp := Suc (Suc ep))))) (case_register hp (Suc (Suc ep)) vp (Suc sp)) 0 (Con 0) 
-            (assembly_map cd (h (Suc (Suc (vs vp))))))" 
-    by (auto simp add: numeral_def)
+    Some (AAddA 2 (Reg Hp))" by (simp del: add_2_eq_Suc)
+  ultimately have "iter_evala (assemble_code cd) 19 (AS (case_register (assm_hp cd h) 
+    (assemble_env e) (assemble_vals vs) (assm_stk cd sh)) (case_register hp ep (Suc (Suc vp)) 
+      (Suc sp)) 0 (Con 0) (assembly_map cd (Suc pc))) = Some (AS (case_register (assm_hp cd h) 
+        (assemble_env (e(ep := vs (Suc vp), Suc ep := h (Suc (vs vp))))) (assemble_vals vs) 
+          (assm_stk cd (sh(sp := Suc (Suc ep))))) (case_register hp (Suc (Suc ep)) vp (Suc sp)) 0 
+            (Con 0) (assembly_map cd (h (Suc (Suc (vs vp))))))" 
+    by (auto simp add: numeral_def assemble_vals_def)
   thus ?case by auto
 qed
 
@@ -677,10 +710,10 @@ proof (induction \<Sigma>\<^sub>u \<Sigma>\<^sub>u' rule: iter.induct)
 next
   case (iter_step \<Sigma>\<^sub>u \<Sigma>\<^sub>u' \<Sigma>\<^sub>u'')
   then obtain n where "iter_evala (assemble_code cd\<^sub>b) n (assm_state cd\<^sub>b \<Sigma>\<^sub>u) = 
-    Some (assm_state cd\<^sub>b \<Sigma>\<^sub>u')" by fastforce
+    Some (assm_state cd\<^sub>b \<Sigma>\<^sub>u')" by (metis correcta)
   moreover from iter_step obtain m where "
     iter_evala (assemble_code cd\<^sub>b) m (assm_state cd\<^sub>b \<Sigma>\<^sub>u') = Some (assm_state cd\<^sub>b \<Sigma>\<^sub>u'')" 
-      by fastforce
+    by (metis preserve_restructure)
   ultimately have "iter_evala (assemble_code cd\<^sub>b) (n + m) (assm_state cd\<^sub>b \<Sigma>\<^sub>u) = 
     Some (assm_state cd\<^sub>b \<Sigma>\<^sub>u'')" by simp
   thus ?case by blast
