14MachineCode/Disassemble.thy
@@ -19,6 +19,11 @@ primrec pseudoreg_size :: "pseudoreg \<Rightarrow> nat" where
 | "pseudoreg_size PC = 1"
 | "pseudoreg_size (Con k) = 1"
 
+fun pseudoreg_map :: "pseudoreg \<times> nat \<Rightarrow> nat" where
+  "pseudoreg_map (Reg r, x) = 4 * x + register_offset r"
+| "pseudoreg_map (PC, x) = x"
+| "pseudoreg_map (Con k, x) = x"
+
 fun disassemble' :: "assm \<Rightarrow> mach" where
   "disassemble' (AMov (Reg r)) = MOV R5 (register_map r)"
 | "disassemble' (AMov PC) = MVP R5"
@@ -26,6 +31,7 @@ fun disassemble' :: "assm \<Rightarrow> mach" where
 | "disassemble' (AGetA r t) = LOD R5 (register_map r)"
 | "disassemble' (AGet r t) = LOD R5 (register_map r)"
 | "disassemble' (APutA r) = STO (register_map r) R5"
+| "disassemble' (APutPC r k) = STI (register_map r) k"
 | "disassemble' (APut r (Reg r')) = STO (register_map r) (register_map r')"
 | "disassemble' (APut r PC) = undefined"
 | "disassemble' (APut r (Con k)) = STI (register_map r) k"
@@ -45,8 +51,8 @@ fun unmap_mem' :: "nat \<Rightarrow> register \<times> nat" where
 | "unmap_mem' (Suc (Suc (Suc 0))) = (Stk, 0)"
 | "unmap_mem' (Suc (Suc (Suc (Suc x)))) = (case unmap_mem' x of (a, b) \<Rightarrow> (a, Suc b))"
 
-definition unmap_mem :: "(register \<Rightarrow> nat \<Rightarrow> nat) \<Rightarrow> nat \<Rightarrow> nat" where
-  "unmap_mem m x = (case unmap_mem' x of (r, p) \<Rightarrow> m r p)"
+definition unmap_mem :: "(register \<Rightarrow> nat \<Rightarrow> pseudoreg \<times> nat) \<Rightarrow> nat \<Rightarrow> nat" where
+  "unmap_mem m x = (case unmap_mem' x of (r, p) \<Rightarrow> pseudoreg_map (m r p))"
 
 fun inv_register_map :: "(register \<Rightarrow> nat) \<Rightarrow> nat \<Rightarrow> pseudoreg \<Rightarrow> reg \<Rightarrow> nat" where
   "inv_register_map rs a t R1 = rs Hp * 4"
@@ -158,10 +164,6 @@ qed (simp_all add: numeral_def)
 lemma [simp]: "inv_register_map (ps(r := k)) a act R5 = inv_register_map ps a act R5"
   by (induction act) simp_all
 
-lemma [simp]: "(unmap_mem mem)(inv_register_map ps a act (register_map r) := k) = 
-    unmap_mem (mem_upd mem r (ps r) k)"
-  by (rule, induction r) (auto simp add: unmap_mem_def split: prod.splits)
-
 lemma [simp]: "inv_register_map (ps(r := ps r + k)) a act = 
   ((inv_register_map ps a act)
     (register_map r := inv_register_map ps a act (register_map r) + 4 * k))"
@@ -212,7 +214,8 @@ proof
   qed simp_all
 qed
 
-lemma [simp]: "unmap_mem mem (inv_register_map ps a (Reg r) (register_map r)) = mem r (ps r)"
+lemma [simp]: "unmap_mem mem (inv_register_map ps a (Reg r) (register_map r)) = 
+    pseudoreg_map (mem r (ps r))"
   by (induction r) (simp_all add: unmap_mem_def split: prod.splits)
 
 lemma [simp]: "((inv_register_map ps a PC)(R5 := 0)) = inv_register_map ps 0 (Con 0)"
@@ -222,8 +225,15 @@ proof
     by (induction x) simp_all
 qed
 
-lemma [simp]: "unmap_mem mem (a * 4 + register_offset m) = mem m a"
-  by (simp add: unmap_mem_def)
+lemma [simp]: "mem m a = (t, b) \<Longrightarrow> 
+  (inv_register_map ps a (Reg m))(R5 := pseudoreg_map (mem m (ps m))) = inv_register_map ps b t"
+proof
+  fix x
+  assume "mem m a = (t, b)"
+  thus "((inv_register_map ps a (Reg m))(R5 := pseudoreg_map (mem m (ps m)))) x = 
+    inv_register_map ps b t x"
+    apply (induction ps b t x rule: inv_register_map.induct) 
+    apply simp_all
 
 lemma [simp]: "lookup cd pc = Some op \<Longrightarrow> disassemble cd ! pc = disassemble' op"
 proof (induction cd)
@@ -250,7 +260,7 @@ next
     MS ((inv_register_map ps a act)(R5 := k)) (unmap_mem mem) pc" by simp
   thus ?case by (simp add: inv_reg_map_con)
 next
-  case (eva_geta cd pc m t mem ps a)  
+  case (eva_geta cd pc m t mem a b ps)  
   hence "disassemble cd ! pc = LOD R5 (register_map m)" by simp
   hence "disassemble cd \<tturnstile> MS (inv_register_map ps a (Reg m)) (unmap_mem mem) (Suc pc) \<leadsto>\<^sub>m
     MS ((inv_register_map ps a (Reg m))(R5 := (unmap_mem mem) ((inv_register_map ps a (Reg m)) 
@@ -270,7 +280,10 @@ next
     MS (inv_register_map ps a act) ((unmap_mem mem)(inv_register_map ps a act (register_map r) := 
       inv_register_map ps a act R5)) pc" by (metis evm_sto)
 
-  thus ?case apply (cases act) by simp_all
+  thus ?case by simp
+next
+  case (eva_putp cd pc r k mem ps a act)
+  thus ?case by simp
 next
   case (eva_putr cd pc r r' mem ps a act)
   hence "disassemble cd ! pc = STO (register_map r) (register_map r')" by simp
@@ -332,9 +345,9 @@ lemma [simp]: "unmap_mem' 7 = (Stk, 1)"
 lemma [dest]: "unmap_mem' x = (Stk, Suc 0) \<Longrightarrow> x = 7"
   by (induction x rule: unmap_mem'.induct) (auto split: prod.splits)
 
-lemma [simp]: "unmap_mem (case_register nmem nmem nmem (nmem(0 := 0, Suc 0 := 0))) = 
-    (nmem(3 := 0, 7 := 0))"
-  by rule (auto simp add: unmap_mem_def split: prod.splits register.splits)
+lemma [simp]: "unmap_mem (case_register nmem nmem nmem 
+    (nmem(0 := (undefined, 0), Suc 0 := (undefined, 0)))) = (nmem(3 := 0, 7 := 0))"
+  by rule (autox simp add: unmap_mem_def split: prod.splits register.splits)
 
 lemma [simp]: "unmap_mem (case_register h e v s) 2 = v 0"
   by (simp add: unmap_mem_def numeral_def)
